feat: define first projection and prove correct
Define the first Futamura projection and prove that the compiled program
yielded behaves identically to the source.

Futamura/Projections.lean
@@ -25,9 +25,24 @@ structure Compiler {I O : Type} (S T : Lang) where
   correct: ∀ (p : S.Prog I O) (x : I), S.eval p x = T.eval (T.eval prog p) x
 
 /-- A specializer (partial evaluator) for `T`: a `T`-program that takes a program expecting a static-dynamic pair and a static input, and produces a residual program over just the dynamic input. -/
-structure Mix {S D O : Type} (T : Lang) where
+structure Mix {St Dy O : Type} (T : Lang) where
   /-- The partial evaluator program. -/
-  prog: T.Prog ((T.Prog (S × D) O) × S) (T.Prog D O)
+  prog: T.Prog ((T.Prog (St × Dy) O) × St) (T.Prog Dy O)
   /-- The residual program is equivalent to the original with the static input fixed. -/
-  correct: ∀ (p : T.Prog (S × D) O) (s : S) (x : D),
+  correct: ∀ (p : T.Prog (St × Dy) O) (s : St) (x : Dy),
     T.eval p (s, x) = T.eval (T.eval prog (p, s)) x
+
+/-- First Futamura projection: specializing an interpreter to a program yields a compiled program. -/
+def projection1 {I O : Type}
+    (S T : Lang) (mix : @Mix (S.Prog I O) I O T) (interp : @Interp I O S T) (p : S.Prog I O) : T.Prog I O :=
+  T.eval mix.prog (interp.prog, p)
+
+/-- The compiled program behaves the same as the source program. -/
+theorem projection1_correct {I O : Type}
+    (S T : Lang) (mix : @Mix (S.Prog I O) I O T)
+    (interp : @Interp I O S T) (p : S.Prog I O)
+    (x : I) :
+    S.eval p x = T.eval (projection1 S T mix interp p) x := by
+  unfold projection1
+  rw [← Mix.correct]
+  rw [← Interp.correct]
